@prefix : <http://www.city.ac.uk/ds/inm713/aaron_altrock/> .
@prefix aa: <http://www.city.ac.uk/ds/inm713/aaron_altrock/> .
@prefix owl: <http://www.w3.org/2002/07/owl#> .
@prefix rdf: <http://www.w3.org/1999/02/22-rdf-syntax-ns#> .
@prefix xml: <http://www.w3.org/XML/1998/namespace> .
@prefix xsd: <http://www.w3.org/2001/XMLSchema#> .
@prefix rdfs: <http://www.w3.org/2000/01/rdf-schema#> .
@base <http://www.city.ac.uk/ds/inm713/aaron_altrock/> .

<http://www.city.ac.uk/ds/inm713/aaron_altrock/> rdf:type owl:Ontology ;
                                                  rdfs:comment "This ontology is to define restaurants and menu items globally." .

#################################################################
#    Object Properties
#################################################################

###  http://www.city.ac.uk/ds/inm713/aaron_altrock/derives
aa:derives rdf:type owl:ObjectProperty ;
           rdfs:subPropertyOf owl:topObjectProperty ;
           rdf:type owl:FunctionalProperty ;
           rdfs:domain aa:menuItem ;
           rdfs:range aa:generic_dish ;
           rdfs:comment "A menu item is derived from a generic dish.  Only one generic dish is derived by a specific venue (e.g. Cheese Pizza cannot be interpreted as two for the same venue)."@en ;
           rdfs:label "derives"@en .


###  http://www.city.ac.uk/ds/inm713/aaron_altrock/follows_in_style_of
aa:follows_in_style_of rdf:type owl:ObjectProperty ;
                       rdfs:subPropertyOf owl:topObjectProperty ;
                       rdfs:domain aa:venue ;
                       rdfs:range aa:venue_style ;
                       rdfs:comment "Venue styles from a particular cuisine or ambience."@en ;
                       rdfs:label "follows in style of"@en .


###  http://www.city.ac.uk/ds/inm713/aaron_altrock/has_city_of
aa:has_city_of rdf:type owl:ObjectProperty ;
               rdfs:domain aa:state ;
               rdfs:range aa:city ;
               rdfs:comment "A state has a city of."@en ;
               rdfs:label "has city of"@en .


###  http://www.city.ac.uk/ds/inm713/aaron_altrock/has_in_city
aa:has_in_city rdf:type owl:ObjectProperty ;
               rdfs:subPropertyOf owl:topObjectProperty ;
               rdf:type owl:FunctionalProperty ;
               rdfs:domain aa:city ;
               rdfs:range aa:venue ;
               rdfs:comment "City has venue.  Only one particular venue of an organisation with a specific post code exists in a city."@en ;
               rdfs:label "has in city"@en .


###  http://www.city.ac.uk/ds/inm713/aaron_altrock/has_ingredient_of
aa:has_ingredient_of rdf:type owl:ObjectProperty ;
                     rdfs:domain aa:menuItem ;
                     rdfs:range aa:ingredient ;
                     rdfs:comment "Defines a specific venue uses which ingridient to produce its specific menu item."@en ;
                     rdfs:label "cooks with"@en .


###  http://www.city.ac.uk/ds/inm713/aaron_altrock/has_state
aa:has_state rdf:type owl:ObjectProperty ;
             rdfs:domain aa:country ;
             rdfs:range aa:state ;
             rdfs:comment "A country has a state."@en ;
             rdfs:label "has state"@en .


###  http://www.city.ac.uk/ds/inm713/aaron_altrock/has_venue_in
aa:has_venue_in rdf:type owl:ObjectProperty ,
                         owl:FunctionalProperty ;
                rdfs:domain aa:organisation ;
                rdfs:range aa:venue ;
                rdfs:comment "An organisation has at least one venue.  Each venue is a specific location."@en ;
                rdfs:label "has venue in"@en .


###  http://www.city.ac.uk/ds/inm713/aaron_altrock/is_derived_from
aa:is_derived_from rdf:type owl:ObjectProperty ;
                   rdfs:subPropertyOf owl:topObjectProperty ;
                   rdf:type owl:FunctionalProperty ;
                   rdfs:domain aa:generic_dish ;
                   rdfs:range aa:menuItem ;
                   rdfs:comment "Is derived from a generic dish into a menu item.  Only one menu item is derived from one generic dish for a specific venue."@en ;
                   rdfs:label "is derived as"@en .


###  http://www.city.ac.uk/ds/inm713/aaron_altrock/is_followed_in_style_by
aa:is_followed_in_style_by rdf:type owl:ObjectProperty ;
                           rdfs:domain aa:venue_style ;
                           rdfs:range aa:venue ;
                           rdfs:comment "Venue follows a style of setting"@en ;
                           rdfs:label "is followed in style by"@en .


###  http://www.city.ac.uk/ds/inm713/aaron_altrock/is_in_country
aa:is_in_country rdf:type owl:ObjectProperty ,
                          owl:FunctionalProperty ;
                 rdfs:domain aa:state ;
                 rdfs:range aa:country ;
                 rdfs:comment "A state belongs to a country.  A state can only beong to one country."@en ;
                 rdfs:label "is in country"@en .


###  http://www.city.ac.uk/ds/inm713/aaron_altrock/is_in_organisation
aa:is_in_organisation rdf:type owl:ObjectProperty ,
                               owl:FunctionalProperty ;
                      rdfs:domain aa:venue ;
                      rdfs:range aa:organisation ;
                      rdfs:comment "A venue is in an organisation.  A venue can only belong to one organisation."@en ;
                      rdfs:label "is in organisation"@en .


###  http://www.city.ac.uk/ds/inm713/aaron_altrock/is_in_state
aa:is_in_state rdf:type owl:ObjectProperty ;
               rdfs:domain aa:city ;
               rdfs:range aa:state ;
               rdfs:comment "A city is in a state."@en ,
                            "A city is in state."@en .


###  http://www.city.ac.uk/ds/inm713/aaron_altrock/is_ingredient_of
aa:is_ingredient_of rdf:type owl:ObjectProperty ;
                    rdfs:domain aa:ingredient ;
                    rdfs:range aa:menuItem ;
                    rdfs:comment "Is ingredient of a menu item."@en ;
                    rdfs:label "is ingredient of"@en .


###  http://www.city.ac.uk/ds/inm713/aaron_altrock/is_sold_by
aa:is_sold_by rdf:type owl:ObjectProperty ,
                       owl:FunctionalProperty ;
              rdfs:domain aa:menuItem ;
              rdfs:range aa:venue ;
              rdfs:comment "A specific menu item is sold by a specific venue.  Only one menu item can be sold by one venue."@en ;
              rdfs:label "is sold by"@en .


###  http://www.city.ac.uk/ds/inm713/aaron_altrock/locates_in
aa:locates_in rdf:type owl:ObjectProperty ,
                       owl:FunctionalProperty ;
              rdfs:domain aa:venue ;
              rdfs:range aa:city ;
              rdfs:comment "Locates in which city."@en ;
              rdfs:label "locates in"@en .


###  http://www.city.ac.uk/ds/inm713/aaron_altrock/sells
aa:sells rdf:type owl:ObjectProperty ,
                  owl:FunctionalProperty ;
         rdfs:domain aa:venue ;
         rdfs:range aa:menuItem ;
         rdfs:comment "sells at a specific venue.  A venue can only sell one menu item of one name."@en ;
         rdfs:label "sells"@en .


#################################################################
#    Data properties
#################################################################

###  http://www.city.ac.uk/ds/inm713/aaron_altrock/address
aa:address rdf:type owl:DatatypeProperty ;
           rdfs:domain aa:venue ;
           rdfs:range xsd:string ;
           rdfs:comment "First line of address of the venue."@en ;
           rdfs:label "Address"@en .


###  http://www.city.ac.uk/ds/inm713/aaron_altrock/cost
aa:cost rdf:type owl:DatatypeProperty ;
        rdfs:domain aa:menuItem ;
        rdfs:range xsd:float ;
        rdfs:comment "Cost of a menu item at a specific venue."@en ;
        rdfs:label "Price"@en .


###  http://www.city.ac.uk/ds/inm713/aaron_altrock/currency
aa:currency rdf:type owl:DatatypeProperty ;
            rdfs:subPropertyOf aa:cost ;
            rdfs:domain aa:country ;
            rdfs:range xsd:string ;
            rdfs:comment "Currency that is charged for the price."@en ;
            rdfs:label "Currency"@en .


###  http://www.city.ac.uk/ds/inm713/aaron_altrock/description
aa:description rdf:type owl:DatatypeProperty ,
                        owl:FunctionalProperty ;
               rdfs:domain aa:menuItem ;
               rdfs:range xsd:string ;
               rdfs:comment "Additional comments included for the menu item at a specific venue.  Only one comment per menu item."@en ;
               rdfs:label "Extra description"@en .


###  http://www.city.ac.uk/ds/inm713/aaron_altrock/postcode
aa:postcode rdf:type owl:DatatypeProperty ;
            rdfs:subPropertyOf aa:address ;
            rdfs:domain aa:venue ;
            rdfs:range xsd:string ;
            rdfs:comment "post code that forms part of an address"@en ;
            rdfs:label "Zip code"@en .


#################################################################
#    Classes
#################################################################

###  http://www.city.ac.uk/ds/inm713/aaron_altrock/city
aa:city rdf:type owl:Class ;
        rdfs:subClassOf aa:state ;
        owl:disjointWith aa:country ,
                         aa:state ;
        rdfs:comment "An urban area within a state."@en ;
        rdfs:label "City"@en .


###  http://www.city.ac.uk/ds/inm713/aaron_altrock/country
aa:country rdf:type owl:Class ;
           owl:disjointWith aa:state ;
           rdfs:comment "Country contains states and cities within."@en ;
           rdfs:label "Country"@en .


###  http://www.city.ac.uk/ds/inm713/aaron_altrock/generic_dish
aa:generic_dish rdf:type owl:Class ;
                owl:disjointWith aa:ingredient ,
                                 aa:menuItem ;
                rdfs:comment "A generally recgonised dish.  A venue cannot produce exactly this generic dish and must be an adaptation of it, and it cannot be an ingredient itself."@en ;
                rdfs:label "Generic dish"@en .


###  http://www.city.ac.uk/ds/inm713/aaron_altrock/ingredient
aa:ingredient rdf:type owl:Class ;
              owl:disjointWith aa:menuItem ;
              rdfs:comment "Ingredients for producing a menu item in an eatery.  An ingredient cannot be a generic dish nor a menu item at a specific venue."@en ;
              rdfs:label "Ingredient"@en .


###  http://www.city.ac.uk/ds/inm713/aaron_altrock/menuItem
aa:menuItem rdf:type owl:Class ;
            rdfs:subClassOf aa:venue ;
            rdfs:comment "A specific dish served in a venue that is an interpretation of a generic dish."@en ;
            rdfs:label "Menu Item"@en .


###  http://www.city.ac.uk/ds/inm713/aaron_altrock/organisation
aa:organisation rdf:type owl:Class ;
                rdfs:comment "An organisation consisting of one or more venues."@en ;
                rdfs:label "Organisation"@en .


###  http://www.city.ac.uk/ds/inm713/aaron_altrock/state
aa:state rdf:type owl:Class ;
         rdfs:subClassOf aa:country ;
         rdfs:comment "A state that forms part of a country."@en ;
         rdfs:label "US state"@en .


###  http://www.city.ac.uk/ds/inm713/aaron_altrock/venue
aa:venue rdf:type owl:Class ;
         rdfs:subClassOf aa:organisation ;
         owl:disjointWith aa:venue_style ;
         rdfs:comment "A venue serving food of a specific location and is part of a wider organisation.  Each venue can be eateries with different styles, serving different menu items."@en ;
         rdfs:label "Eatery venue"@en .


###  http://www.city.ac.uk/ds/inm713/aaron_altrock/venue_style
aa:venue_style rdf:type owl:Class ;
               rdfs:comment "The settings of a venue that represents its ambience or cuisine.  A venue setting cannot be a venue itself e.g. a restaurant cannot be called 'American Restaurant'."@en ;
               rdfs:label "Venue Setting"@en .


#################################################################
#    Individuals
#################################################################

###  http://www.city.ac.uk/ds/inm713/aaron_altrock/American_Restaurant
aa:American_Restaurant rdf:type owl:NamedIndividual ,
                                aa:venue_style ;
                       aa:is_followed_in_style_by aa:MA_2601 ;
                       rdfs:label "American Restaurant"@en .


###  http://www.city.ac.uk/ds/inm713/aaron_altrock/Bend
aa:Bend rdf:type owl:NamedIndividual ,
                 aa:city ;
        aa:has_in_city aa:OR_97701 ;
        aa:is_in_state aa:OR .


###  http://www.city.ac.uk/ds/inm713/aaron_altrock/Bianca_Pizza
aa:Bianca_Pizza rdf:type owl:NamedIndividual ,
                         aa:generic_dish ;
                aa:derives aa:OR_97701_Bianca_Pizza ;
                rdfs:label "Bianca Pizza"@en .


###  http://www.city.ac.uk/ds/inm713/aaron_altrock/Cheese_Pizza
aa:Cheese_Pizza rdf:type owl:NamedIndividual ,
                         aa:generic_dish ;
                aa:derives aa:MA_2601_Cheese_Pizza ,
                           aa:OR_97701_Cheese_Pizza ;
                rdfs:label "Cheese Pizza"@en .


###  http://www.city.ac.uk/ds/inm713/aaron_altrock/French_Restaurant
aa:French_Restaurant rdf:type owl:NamedIndividual ,
                              aa:venue_style ;
                     aa:is_followed_in_style_by aa:MA_2601 ;
                     rdfs:label "French Restaurant"@en .


###  http://www.city.ac.uk/ds/inm713/aaron_altrock/Hyannis
aa:Hyannis rdf:type owl:NamedIndividual ,
                    aa:city ;
           aa:has_in_city aa:MA_2601 ;
           aa:is_in_state aa:MA .


###  http://www.city.ac.uk/ds/inm713/aaron_altrock/Little_Pizza_Paradise
aa:Little_Pizza_Paradise rdf:type owl:NamedIndividual ,
                                  aa:organisation ;
                         aa:has_venue_in aa:OR_97701 ;
                         rdfs:label "Little Pizza Paradise"@en .


###  http://www.city.ac.uk/ds/inm713/aaron_altrock/MA
aa:MA rdf:type owl:NamedIndividual ,
               aa:state ;
      aa:has_city_of aa:Hyannis ;
      aa:is_in_country aa:US ;
      rdfs:comment "A state in North East of the US."@en ;
      rdfs:label "Massachusetts"@en .


###  http://www.city.ac.uk/ds/inm713/aaron_altrock/MA_2601
aa:MA_2601 rdf:type owl:NamedIndividual ,
                    aa:venue ;
           aa:follows_in_style_of aa:American_Restaurant ,
                                  aa:French_Restaurant ,
                                  aa:Seafood_Restaurant ;
           aa:is_in_organisation aa:Roadhouse_Cafe ;
           aa:locates_in aa:Hyannis ;
           aa:sells aa:Cheese_Pizza ;
           aa:address "478 South St"@en ;
           aa:postcode 2601 ;
           rdfs:label "Roadhouse Cafe"@en .


###  http://www.city.ac.uk/ds/inm713/aaron_altrock/MA_2601_Cheese_Pizza
aa:MA_2601_Cheese_Pizza rdf:type owl:NamedIndividual ,
                                 aa:menuItem ;
                        aa:has_ingredient_of aa:cheese ;
                        aa:is_derived_from aa:Cheese_Pizza ;
                        aa:sells aa:MA_2601 ;
                        aa:cost "8.95"@en ;
                        rdfs:comment "Cheese Pizza served at Roadhouse Cafe"@en ;
                        rdfs:label "Cheese Pizza from Roundhouse Cafe"@en .


###  http://www.city.ac.uk/ds/inm713/aaron_altrock/OR
aa:OR rdf:type owl:NamedIndividual ,
               aa:state ;
      aa:has_city_of aa:Bend ;
      aa:is_in_country aa:US ;
      rdfs:comment "A state in the North West of the US."@en ;
      rdfs:label "Oregon"@en .


###  http://www.city.ac.uk/ds/inm713/aaron_altrock/OR_97701
aa:OR_97701 rdf:type owl:NamedIndividual ,
                     aa:venue ;
            aa:follows_in_style_of aa:Pizza_Place ;
            aa:is_in_organisation aa:Little_Pizza_Paradise ;
            aa:locates_in aa:Bend ;
            aa:sells aa:Bianca_Pizza ,
                     aa:Cheese_Pizza ;
            aa:address "Cascade Village Mall Across From Target"@en ;
            aa:postcode 97701 ;
            rdfs:label "Little Pizza Paradise"@en .


###  http://www.city.ac.uk/ds/inm713/aaron_altrock/OR_97701_Bianca_Pizza
aa:OR_97701_Bianca_Pizza rdf:type owl:NamedIndividual ,
                                  aa:menuItem ;
                         aa:is_derived_from aa:Bianca_Pizza ;
                         aa:is_sold_by aa:OR_97701 ;
                         aa:cost "22.50"@en ;
                         rdfs:comment "Bianca Pizza served at Little Pizza Paradise"@en ;
                         rdfs:label "Bianca Pizza from Little Pizza Paradise with zip code 97701"@en .


###  http://www.city.ac.uk/ds/inm713/aaron_altrock/OR_97701_Cheese_Pizza
aa:OR_97701_Cheese_Pizza rdf:type owl:NamedIndividual ,
                                  aa:menuItem ;
                         aa:has_ingredient_of aa:cheese ;
                         aa:is_derived_from aa:Cheese_Pizza ;
                         aa:is_sold_by aa:OR_97701 ;
                         aa:cost "18.95"@en ;
                         rdfs:comment "Cheese Pizza served at Little Pizza Paradise"@en ;
                         rdfs:label "Cheese Pizza from Little Pizza Paradise with zip code 97701"@en .


###  http://www.city.ac.uk/ds/inm713/aaron_altrock/Pizza_Place
aa:Pizza_Place rdf:type owl:NamedIndividual ,
                        aa:venue_style ;
               aa:is_followed_in_style_by aa:OR_97701 ;
               rdfs:label "Pizza Place"@en .


###  http://www.city.ac.uk/ds/inm713/aaron_altrock/Roadhouse_Cafe
aa:Roadhouse_Cafe rdf:type owl:NamedIndividual ,
                           aa:organisation ;
                  aa:has_venue_in aa:MA_2601 ;
                  rdfs:label "Roundhouse Cafe"@en .


###  http://www.city.ac.uk/ds/inm713/aaron_altrock/Seafood_Restaurant
aa:Seafood_Restaurant rdf:type owl:NamedIndividual ,
                               aa:venue_style ;
                      aa:is_followed_in_style_by aa:MA_2601 ;
                      rdfs:label "Seafood Restaurant"@en .


###  http://www.city.ac.uk/ds/inm713/aaron_altrock/US
aa:US rdf:type owl:NamedIndividual ,
               aa:country ;
      aa:has_state aa:MA ,
                   aa:OR ;
      aa:currency "USD"@en ;
      rdfs:comment "US as the country with US states and cities being subclasses of this."@en ;
      rdfs:label "United States of America"@en .


###  http://www.city.ac.uk/ds/inm713/aaron_altrock/cheese
aa:cheese rdf:type owl:NamedIndividual ,
                   aa:ingredient ;
          aa:is_ingredient_of aa:Cheese_Pizza .


#################################################################
#    General axioms
#################################################################

[ rdf:type owl:AllDifferent ;
  owl:distinctMembers ( aa:MA_2601_Cheese_Pizza
                        aa:OR_97701_Cheese_Pizza
                      )
] .


###  Generated by the OWL API (version 4.5.9.2019-02-01T07:24:44Z) https://github.com/owlcs/owlapi
